examples/cannon/CannonAll.v
@@ -1,5 +1,6 @@
 Require Import HoareDef STB CannonRA CannonMain0 CannonMain1 Cannon0 Cannon1.
 Require Import Cannon01proof CannonMain01proof.
+Require Import ModSemFacts SimModSemFacts.
 Require Import Coqlib.
 Require Import ImpPrelude.
 Require Import Skeleton.
@@ -22,8 +23,42 @@ Section PROOF.
   Section ERASE.
     Variable num_fire: nat.
 
+    (* Let smd0 := Cannon1.SCannon.
+    Let stb0 := fun sk => to_closed_stb (SMod.get_stb smd0 sk).
+    Let src0 := SMod.to_src smd0.
+    Let tgt0 := (SMod.to_tgt stb0) smd0.
+
+    Let smd1 := CannonMain1.SMain num_fire.
+    Let stb1 := fun sk => to_closed_stb (SMod.get_stb smd1 sk).
+    Let src1 := SMod.to_src smd1.
+    Let tgt1 := (SMod.to_tgt stb1) smd1. *)
+
+
+    Let smd2 := SMod.add Cannon1.SCannon (CannonMain1.SMain num_fire).
+    Let stb2 := fun sk => to_closed_stb (SMod.get_stb smd2 sk).
+    Let src2 := SMod.to_src smd2.
+    Let tgt2 := (SMod.to_tgt stb2) smd2.
+
+    Theorem cannon_erase_spec:
+      refines_closed tgt2 src2. 
+    Proof.
+      eapply adequacy_type_closed with (entry_r := GRA.embed Ball).
+      { g_wf_tac. des_ifs. eapply BallReady_wf. }
+      { unfold to_closed_stb. cbn. i. ss. clarify.
+        exists tt. split; ss.
+        { iIntros "H". iSplits; ss. }
+        { split; ss. ii. iPureIntro. i. des. auto. }
+      }
+    Qed.
+
+
+    
+  (* Definition get_stb_list (mds: list SMod.t): Sk.t -> alist gname fspec :=
+    fun sk => map (map_snd fsb_fspec) (flat_map (SModSem.fnsems ∘ (flip SMod.get_modsem sk)) mds).
+
     Let smd := [Cannon1.SCannon; CannonMain1.SMain num_fire].
-    Let stb := fun sk => to_closed_stb (SMod.get_stb smd sk).
+    Let stb := fun sk => to_closed_stb (get_stb_list smd sk).
+    (* Let stb := fun sk => to_closed_stb (concat (List.map (fun f => f sk) (List.map SMod.get_stb smd))). *)
     Let prog_src := List.map SMod.to_src smd.
     Let prog_tgt := List.map (SMod.to_tgt stb) smd.
 
@@ -40,15 +75,54 @@ Section PROOF.
         { split; ss. ii. iPureIntro. i. des. auto. }
       }
     Qed.
+
+    Theorem cannon_erase_spec:
+      refines_closed
+        (Mod.add_list prog_tgt)
+        (Mod.add_list prog_src).
+    Proof.
+      eapply adequacy_type_closed with (entry_r := GRA.embed Ball).
+      { g_wf_tac. eapply BallReady_wf. }
+      { unfold to_closed_stb. cbn. i. ss. clarify.
+        exists tt. split; ss.
+        { iIntros "H". iSplits; ss. }
+        { split; ss. ii. iPureIntro. i. des. auto. }
+      }
+    Qed. *)
   End ERASE.
+
+  Lemma add_to_src
+    (m1 m2 : SMod.t)
+  :
+    SMod.to_src (SMod.add m1 m2) = Mod.add (SMod.to_src m1) (SMod.to_src m2)
+  .
+  Proof. Admitted.
+
+  Lemma add_to_tgt
+  (m1 m2 : SMod.t)
+  stb
+:
+  SMod.to_tgt stb (SMod.add m1 m2) = Mod.add (SMod.to_tgt stb m1) (SMod.to_tgt stb m2)
+.
+Proof. Admitted.
 
   Theorem cannon_1_correct:
     refines_closed
       (Mod.add_list ([Cannon0.Cannon; CannonMain0.Main 1]))
+      (* (SMod.to_src (SMod.add SCannon (SMain 1))). *)
       (Mod.add_list (List.map SMod.to_src [SCannon; SMain 1])).
   Proof.
-    etrans; [|eapply cannon_erase_spec].
-    { eapply refines_close. eapply refines2_cons.
+    s.
+    etrans.
+    2: {
+      etrans. 
+      { eapply cannon_erase_spec. }
+      { rewrite add_to_src. unfold refines_closed. ii. apply PR. }
+      }
+    (* etrans; [|eapply cannon_erase_spec]. *)
+    { eapply refines_close.
+      rewrite add_to_tgt.
+      eapply refines_add.
       { eapply Cannon01proof.correct. }
       { eapply CannonMain01proof.correct. i. ss. }
     }
